plugin/printer.ml
@@ -3,8 +3,220 @@ type bool =
 | True
 | False
 
+type nat =
+| O
+| S of nat
+
+type ('a, 'b) prod =
+| Pair of 'a * 'b
+
+type comparison =
+| Eq
+| Lt
+| Gt
+
+(** val compOpp : comparison -> comparison **)
+
+let compOpp = function
+| Eq -> Eq
+| Lt -> Gt
+| Gt -> Lt
+
+module Coq__1 = struct
+ (** val add : nat -> nat -> nat **)
+
+ let rec add n0 m =
+   match n0 with
+   | O -> m
+   | S p -> S (add p m)
+end
+include Coq__1
+
+type positive =
+| XI of positive
+| XO of positive
+| XH
+
+type n =
+| N0
+| Npos of positive
+
+type z =
+| Z0
+| Zpos of positive
+| Zneg of positive
+
+module Pos =
+ struct
+  (** val succ : positive -> positive **)
+
+  let rec succ = function
+  | XI p -> XO (succ p)
+  | XO p -> XI p
+  | XH -> XO XH
+
+  (** val add : positive -> positive -> positive **)
+
+  let rec add x y =
+    match x with
+    | XI p ->
+      (match y with
+       | XI q -> XO (add_carry p q)
+       | XO q -> XI (add p q)
+       | XH -> XO (succ p))
+    | XO p ->
+      (match y with
+       | XI q -> XI (add p q)
+       | XO q -> XO (add p q)
+       | XH -> XI p)
+    | XH -> (match y with
+             | XI q -> XO (succ q)
+             | XO q -> XI q
+             | XH -> XO XH)
+
+  (** val add_carry : positive -> positive -> positive **)
+
+  and add_carry x y =
+    match x with
+    | XI p ->
+      (match y with
+       | XI q -> XI (add_carry p q)
+       | XO q -> XO (add_carry p q)
+       | XH -> XI (succ p))
+    | XO p ->
+      (match y with
+       | XI q -> XO (add_carry p q)
+       | XO q -> XI (add p q)
+       | XH -> XO (succ p))
+    | XH ->
+      (match y with
+       | XI q -> XI (succ q)
+       | XO q -> XO (succ q)
+       | XH -> XI XH)
+
+  (** val pred_double : positive -> positive **)
+
+  let rec pred_double = function
+  | XI p -> XI (XO p)
+  | XO p -> XI (pred_double p)
+  | XH -> XH
+
+  (** val mul : positive -> positive -> positive **)
+
+  let rec mul x y =
+    match x with
+    | XI p -> add y (XO (mul p y))
+    | XO p -> XO (mul p y)
+    | XH -> y
+
+  (** val compare_cont : comparison -> positive -> positive -> comparison **)
+
+  let rec compare_cont r x y =
+    match x with
+    | XI p ->
+      (match y with
+       | XI q -> compare_cont r p q
+       | XO q -> compare_cont Gt p q
+       | XH -> Gt)
+    | XO p ->
+      (match y with
+       | XI q -> compare_cont Lt p q
+       | XO q -> compare_cont r p q
+       | XH -> Gt)
+    | XH -> (match y with
+             | XH -> r
+             | _ -> Lt)
+
+  (** val compare : positive -> positive -> comparison **)
+
+  let compare =
+    compare_cont Eq
+
+  (** val eqb : positive -> positive -> bool **)
+
+  let rec eqb p q =
+    match p with
+    | XI p0 -> (match q with
+                | XI q0 -> eqb p0 q0
+                | _ -> False)
+    | XO p0 -> (match q with
+                | XO q0 -> eqb p0 q0
+                | _ -> False)
+    | XH -> (match q with
+             | XH -> True
+             | _ -> False)
+
+  (** val iter_op : ('a1 -> 'a1 -> 'a1) -> positive -> 'a1 -> 'a1 **)
+
+  let rec iter_op op p a =
+    match p with
+    | XI p0 -> op a (iter_op op p0 (op a a))
+    | XO p0 -> iter_op op p0 (op a a)
+    | XH -> a
+
+  (** val to_nat : positive -> nat **)
+
+  let to_nat x =
+    iter_op Coq__1.add x (S O)
+
+  (** val of_succ_nat : nat -> positive **)
+
+  let rec of_succ_nat = function
+  | O -> XH
+  | S x -> succ (of_succ_nat x)
+ end
+
+module N =
+ struct
+  (** val of_nat : nat -> n **)
+
+  let of_nat = function
+  | O -> N0
+  | S n' -> Npos (Pos.of_succ_nat n')
+ end
+
 type ascii =
 | Ascii of bool * bool * bool * bool * bool * bool * bool * bool
+
+(** val zero : ascii **)
+
+let zero =
+  Ascii (False, False, False, False, False, False, False, False)
+
+(** val one : ascii **)
+
+let one =
+  Ascii (True, False, False, False, False, False, False, False)
+
+(** val shift : bool -> ascii -> ascii **)
+
+let shift c = function
+| Ascii (a1, a2, a3, a4, a5, a6, a7, _) ->
+  Ascii (c, a1, a2, a3, a4, a5, a6, a7)
+
+(** val ascii_of_pos : positive -> ascii **)
+
+let ascii_of_pos =
+  let rec loop n0 p =
+    match n0 with
+    | O -> zero
+    | S n' ->
+      (match p with
+       | XI p' -> shift True (loop n' p')
+       | XO p' -> shift False (loop n' p')
+       | XH -> one)
+  in loop (S (S (S (S (S (S (S (S O))))))))
+
+(** val ascii_of_N : n -> ascii **)
+
+let ascii_of_N = function
+| N0 -> zero
+| Npos p -> ascii_of_pos p
+
+(** val ascii_of_nat : nat -> ascii **)
+
+let ascii_of_nat a =
+  ascii_of_N (N.of_nat a)
 
 type string =
 | EmptyString
@@ -16,6 +228,200 @@ let rec append s1 s2 =
   match s1 with
   | EmptyString -> s2
   | String (c, s1') -> String (c, (append s1' s2))
+
+module Z =
+ struct
+  (** val double : z -> z **)
+
+  let double = function
+  | Z0 -> Z0
+  | Zpos p -> Zpos (XO p)
+  | Zneg p -> Zneg (XO p)
+
+  (** val succ_double : z -> z **)
+
+  let succ_double = function
+  | Z0 -> Zpos XH
+  | Zpos p -> Zpos (XI p)
+  | Zneg p -> Zneg (Pos.pred_double p)
+
+  (** val pred_double : z -> z **)
+
+  let pred_double = function
+  | Z0 -> Zneg XH
+  | Zpos p -> Zpos (Pos.pred_double p)
+  | Zneg p -> Zneg (XI p)
+
+  (** val pos_sub : positive -> positive -> z **)
+
+  let rec pos_sub x y =
+    match x with
+    | XI p ->
+      (match y with
+       | XI q -> double (pos_sub p q)
+       | XO q -> succ_double (pos_sub p q)
+       | XH -> Zpos (XO p))
+    | XO p ->
+      (match y with
+       | XI q -> pred_double (pos_sub p q)
+       | XO q -> double (pos_sub p q)
+       | XH -> Zpos (Pos.pred_double p))
+    | XH ->
+      (match y with
+       | XI q -> Zneg (XO q)
+       | XO q -> Zneg (Pos.pred_double q)
+       | XH -> Z0)
+
+  (** val add : z -> z -> z **)
+
+  let add x y =
+    match x with
+    | Z0 -> y
+    | Zpos x' ->
+      (match y with
+       | Z0 -> x
+       | Zpos y' -> Zpos (Pos.add x' y')
+       | Zneg y' -> pos_sub x' y')
+    | Zneg x' ->
+      (match y with
+       | Z0 -> x
+       | Zpos y' -> pos_sub y' x'
+       | Zneg y' -> Zneg (Pos.add x' y'))
+
+  (** val opp : z -> z **)
+
+  let opp = function
+  | Z0 -> Z0
+  | Zpos x0 -> Zneg x0
+  | Zneg x0 -> Zpos x0
+
+  (** val sub : z -> z -> z **)
+
+  let sub m n0 =
+    add m (opp n0)
+
+  (** val mul : z -> z -> z **)
+
+  let mul x y =
+    match x with
+    | Z0 -> Z0
+    | Zpos x' ->
+      (match y with
+       | Z0 -> Z0
+       | Zpos y' -> Zpos (Pos.mul x' y')
+       | Zneg y' -> Zneg (Pos.mul x' y'))
+    | Zneg x' ->
+      (match y with
+       | Z0 -> Z0
+       | Zpos y' -> Zneg (Pos.mul x' y')
+       | Zneg y' -> Zpos (Pos.mul x' y'))
+
+  (** val compare : z -> z -> comparison **)
+
+  let compare x y =
+    match x with
+    | Z0 -> (match y with
+             | Z0 -> Eq
+             | Zpos _ -> Lt
+             | Zneg _ -> Gt)
+    | Zpos x' -> (match y with
+                  | Zpos y' -> Pos.compare x' y'
+                  | _ -> Gt)
+    | Zneg x' ->
+      (match y with
+       | Zneg y' -> compOpp (Pos.compare x' y')
+       | _ -> Lt)
+
+  (** val leb : z -> z -> bool **)
+
+  let leb x y =
+    match compare x y with
+    | Gt -> False
+    | _ -> True
+
+  (** val ltb : z -> z -> bool **)
+
+  let ltb x y =
+    match compare x y with
+    | Lt -> True
+    | _ -> False
+
+  (** val eqb : z -> z -> bool **)
+
+  let eqb x y =
+    match x with
+    | Z0 -> (match y with
+             | Z0 -> True
+             | _ -> False)
+    | Zpos p -> (match y with
+                 | Zpos q -> Pos.eqb p q
+                 | _ -> False)
+    | Zneg p -> (match y with
+                 | Zneg q -> Pos.eqb p q
+                 | _ -> False)
+
+  (** val to_nat : z -> nat **)
+
+  let to_nat = function
+  | Zpos p -> Pos.to_nat p
+  | _ -> O
+
+  (** val pos_div_eucl : positive -> z -> (z, z) prod **)
+
+  let rec pos_div_eucl a b =
+    match a with
+    | XI a' ->
+      let Pair (q, r) = pos_div_eucl a' b in
+      let r' = add (mul (Zpos (XO XH)) r) (Zpos XH) in
+      (match ltb r' b with
+       | True -> Pair ((mul (Zpos (XO XH)) q), r')
+       | False -> Pair ((add (mul (Zpos (XO XH)) q) (Zpos XH)), (sub r' b)))
+    | XO a' ->
+      let Pair (q, r) = pos_div_eucl a' b in
+      let r' = mul (Zpos (XO XH)) r in
+      (match ltb r' b with
+       | True -> Pair ((mul (Zpos (XO XH)) q), r')
+       | False -> Pair ((add (mul (Zpos (XO XH)) q) (Zpos XH)), (sub r' b)))
+    | XH ->
+      (match leb (Zpos (XO XH)) b with
+       | True -> Pair (Z0, (Zpos XH))
+       | False -> Pair ((Zpos XH), Z0))
+
+  (** val div_eucl : z -> z -> (z, z) prod **)
+
+  let div_eucl a b =
+    match a with
+    | Z0 -> Pair (Z0, Z0)
+    | Zpos a' ->
+      (match b with
+       | Z0 -> Pair (Z0, a)
+       | Zpos _ -> pos_div_eucl a' b
+       | Zneg b' ->
+         let Pair (q, r) = pos_div_eucl a' (Zpos b') in
+         (match r with
+          | Z0 -> Pair ((opp q), Z0)
+          | _ -> Pair ((opp (add q (Zpos XH))), (add b r))))
+    | Zneg a' ->
+      (match b with
+       | Z0 -> Pair (Z0, a)
+       | Zpos _ ->
+         let Pair (q, r) = pos_div_eucl a' b in
+         (match r with
+          | Z0 -> Pair ((opp q), Z0)
+          | _ -> Pair ((opp (add q (Zpos XH))), (sub b r)))
+       | Zneg b' ->
+         let Pair (q, r) = pos_div_eucl a' (Zpos b') in Pair (q, (opp r)))
+
+  (** val div : z -> z -> z **)
+
+  let div a b =
+    let Pair (q, _) = div_eucl a b in q
+
+  (** val modulo : z -> z -> z **)
+
+  let modulo a b =
+    let Pair (_, r) = div_eucl a b in r
+ end
 
 type goTy =
 | GTInt
@@ -165,4 +571,49 @@ let rec print_ty = function
     (append (print_ty k)
       (append (String ((Ascii (True, False, True, True, True, False, True,
         False)), EmptyString)) (print_ty v)))
-| GTNamed n -> n
+| GTNamed n0 -> n0
+
+(** val dec_digit : nat -> ascii **)
+
+let dec_digit n0 =
+  ascii_of_nat
+    (add (S (S (S (S (S (S (S (S (S (S (S (S (S (S (S (S (S (S (S (S (S (S (S
+      (S (S (S (S (S (S (S (S (S (S (S (S (S (S (S (S (S (S (S (S (S (S (S (S
+      (S O)))))))))))))))))))))))))))))))))))))))))))))))) n0)
+
+(** val z_digits : nat -> z -> string -> string **)
+
+let rec z_digits fuel z0 acc =
+  match fuel with
+  | O -> acc
+  | S f ->
+    let d = dec_digit (Z.to_nat (Z.modulo z0 (Zpos (XO (XI (XO XH)))))) in
+    (match Z.eqb (Z.div z0 (Zpos (XO (XI (XO XH))))) Z0 with
+     | True -> String (d, acc)
+     | False ->
+       z_digits f (Z.div z0 (Zpos (XO (XI (XO XH))))) (String (d, acc)))
+
+(** val print_Z : z -> string **)
+
+let print_Z z0 =
+  match Z.eqb z0 Z0 with
+  | True ->
+    String ((Ascii (False, False, False, False, True, True, False, False)),
+      EmptyString)
+  | False ->
+    (match Z.ltb z0 Z0 with
+     | True ->
+       append (String ((Ascii (True, False, True, True, False, True, False,
+         False)), EmptyString))
+         (z_digits (S (S (S (S (S (S (S (S (S (S (S (S (S (S (S (S (S (S (S
+           (S (S (S (S (S (S (S (S (S (S (S (S (S (S (S (S (S (S (S (S (S (S
+           (S (S (S (S (S (S (S (S (S (S (S (S (S (S (S (S (S (S (S (S (S (S
+           (S
+           O))))))))))))))))))))))))))))))))))))))))))))))))))))))))))))))))
+           (Z.opp z0) EmptyString)
+     | False ->
+       z_digits (S (S (S (S (S (S (S (S (S (S (S (S (S (S (S (S (S (S (S (S
+         (S (S (S (S (S (S (S (S (S (S (S (S (S (S (S (S (S (S (S (S (S (S (S
+         (S (S (S (S (S (S (S (S (S (S (S (S (S (S (S (S (S (S (S (S (S
+         O)))))))))))))))))))))))))))))))))))))))))))))))))))))))))))))))) z0
+         EmptyString)
