printer.mli
@@ -3,14 +3,123 @@ type bool =
 | True
 | False
 
+type nat =
+| O
+| S of nat
+
+type ('a, 'b) prod =
+| Pair of 'a * 'b
+
+type comparison =
+| Eq
+| Lt
+| Gt
+
+val compOpp : comparison -> comparison
+
+val add : nat -> nat -> nat
+
+type positive =
+| XI of positive
+| XO of positive
+| XH
+
+type n =
+| N0
+| Npos of positive
+
+type z =
+| Z0
+| Zpos of positive
+| Zneg of positive
+
+module Pos :
+ sig
+  val succ : positive -> positive
+
+  val add : positive -> positive -> positive
+
+  val add_carry : positive -> positive -> positive
+
+  val pred_double : positive -> positive
+
+  val mul : positive -> positive -> positive
+
+  val compare_cont : comparison -> positive -> positive -> comparison
+
+  val compare : positive -> positive -> comparison
+
+  val eqb : positive -> positive -> bool
+
+  val iter_op : ('a1 -> 'a1 -> 'a1) -> positive -> 'a1 -> 'a1
+
+  val to_nat : positive -> nat
+
+  val of_succ_nat : nat -> positive
+ end
+
+module N :
+ sig
+  val of_nat : nat -> n
+ end
+
 type ascii =
 | Ascii of bool * bool * bool * bool * bool * bool * bool * bool
+
+val zero : ascii
+
+val one : ascii
+
+val shift : bool -> ascii -> ascii
+
+val ascii_of_pos : positive -> ascii
+
+val ascii_of_N : n -> ascii
+
+val ascii_of_nat : nat -> ascii
 
 type string =
 | EmptyString
 | String of ascii * string
 
 val append : string -> string -> string
+
+module Z :
+ sig
+  val double : z -> z
+
+  val succ_double : z -> z
+
+  val pred_double : z -> z
+
+  val pos_sub : positive -> positive -> z
+
+  val add : z -> z -> z
+
+  val opp : z -> z
+
+  val sub : z -> z -> z
+
+  val mul : z -> z -> z
+
+  val compare : z -> z -> comparison
+
+  val leb : z -> z -> bool
+
+  val ltb : z -> z -> bool
+
+  val eqb : z -> z -> bool
+
+  val to_nat : z -> nat
+
+  val pos_div_eucl : positive -> z -> (z, z) prod
+
+  val div_eucl : z -> z -> (z, z) prod
+
+  val div : z -> z -> z
+
+  val modulo : z -> z -> z
+ end
 
 type goTy =
 | GTInt
@@ -34,3 +143,9 @@ type goTy =
 | GTNamed of string
 
 val print_ty : goTy -> string
+
+val dec_digit : nat -> ascii
+
+val z_digits : nat -> z -> string -> string
+
+val print_Z : z -> string
